with santiago and aseem, some comments on refactoring client_hello, with more to come (hopefully)

src/tls/Handshake.fst
@@ -1,7 +1,7 @@
 (*--build-config
 options:--use_hints --fstar_home ../../../FStar --include ../../../FStar/ucontrib/Platform/fst/ --include ../../../FStar/ucontrib/CoreCrypto/fst/ --include ../../../FStar/examples/low-level/crypto/real --include ../../../FStar/examples/low-level/crypto/spartan --include ../../../FStar/examples/low-level/LowCProvider/fst --include ../../../FStar/examples/low-level/crypto --include ../../libs/ffi --include ../../../FStar/ulib/hyperstack --include ideal-flags;
 --*)
-﻿module Handshake
+module Handshake
 
 open FStar.Heap
 open FStar.HyperHeap
@@ -43,30 +43,55 @@ let hashSize = Hashing.Spec.tagLen
    The F* normalizer will erase debug prints at extraction
    when this flag is set to false. *)
 inline_for_extraction let hs_debug = false
+(* Sketch 
+val Nego.prepareClientOffer: config -> clientOffer
+let Nego.prepareClientOffer cfg =
+  let groups = List.Tot.choose CommonDH.group_of_namedGroup cfg.namedGroups in
+  let cipher_suites = ... in
+  let sigAlgs = ... in
+  let protocol_version = ... in
+  let ext = prepareExtensions protocol_version cipher_suites sigAlgs groups kp in
+*)  
 
 val prepareClientHello: config -> KeySchedule.ks -> HandshakeLog.log -> option ri -> option sessionID -> ST (hs_msg * bytes)
   (requires (fun h -> True))
   (ensures (fun h0 i h1 -> True))
 let prepareClientHello cfg ks log ri sido =
+  (* Who should be generating nonces? KS? *)
   let cr = KeySchedule.ks_client_random ks in
+  (* Negotiation, KeySchedule, Messages: compute serialized key shares *)
+  (* Negotiation should compute the list of groups;
+     KeySchedule should compute the shares from these groups (calling into CommonDH)
+     Messages should do the serialization (calling into CommonDH)\
+  *)
   let kp =
-     (match cfg.maxVer with
+     match cfg.maxVer with
       | TLS_1p3 ->
+         (* This doesn't do any filtering, it's just a map converting to CommonDH.group *)
          let groups = List.Tot.choose CommonDH.group_of_namedGroup cfg.namedGroups in
+         (* Call into KS to generate shares for all of them *)
+         (* TODO: ks_client_13_1rtt_init should take `namedGroup`s, avoiding the above mapping *)
          let gxl = KeySchedule.ks_client_13_1rtt_init ks groups in
+         (* Serialized client shares. Probably should go to HandshakeMessages/Log? *)
          let ser_share (gx:(g:CommonDH.group & CommonDH.share g)) =
            let (| g, gx |) = gx in
            match CommonDH.namedGroup_of_group g with
-           | None -> None // TODO prove from KS that this is impossible
+           | None -> None // TODO: prove from def. of groups above that this is impossible
            | Some ng -> Some (ng, CommonDH.serialize_raw #g gx) in
          let serialized = List.Tot.choose ser_share gxl in
 	       Some (ClientKeyShare serialized)
       | _ ->
       	 let _ = KeySchedule.ks_client_12_init ks in
-	       None)
+	       None
       in
-  let sid = (match sido with | None -> empty_bytes | Some x -> x) in
+  (* Is (Some? sido) in case of resumption? *)
+  let sid = match sido with | None -> empty_bytes | Some x -> x in
+  (* Negotiation: compute offer from configuration *)
+  (* The offer should contain kp *)
   let co = prepareClientOffer cfg in
+  (* Negotiation should do this: it computes the list of extensions to send, gives them back to 
+     Handshake, which then calls into e.g. KeySchedule to turn them into proper extensions that
+     can be serialized *) 
   let ext = prepareExtensions co.co_protocol_version co.co_cipher_suites co.co_safe_resumption co.co_safe_renegotiation co.co_sigAlgs co.co_namedGroups ri kp in
   let ch =
   {ch_protocol_version = co.co_protocol_version;
@@ -76,6 +101,7 @@ let prepareClientHello cfg ks log ri sido =
    ch_raw_cipher_suites = None;
    ch_compressions = co.co_compressions;
    ch_extensions = Some ext;} in
+  (* `@@` has side-effects: it appends the message to the log and returns the message bytes *)
   let chb = log @@ (ClientHello ch) in
   (ClientHello ch, chb)
 
